Add definition and properties of equivalence for LambdaNRA and prove that examples T1l and T1r from the paper are indeed equivalent.

coq/Frontend/LambdaNRA/LambdaAlgExamples.v
@@ -6,7 +6,7 @@ Require Import Morphisms.
 
 Require Import Utils BasicRuntime.
 
-Require Import LambdaAlg LambdaAlgtoNRAEnv.
+Require Import LambdaAlg LambdaAlgEq LambdaAlgtoNRAEnv.
 Require Import TrivialCompiler.
 Import TrivialCompiler.
 
@@ -34,40 +34,139 @@ Section LambdaNRAExamples.
               :: (drec (("name",dstring "Jack")::("age",dnat 40)::("child",child2)::nil))
               :: nil))%string.
 
-  (* T1 : map(λ(a) a.city)(map(λ(p) p.addr)(Q)) == map(λ(p) p.addr.city)(Q) *)
-  Definition T1l Q :=
+  (* T1 : map(λ(a) a.city)(map(λ(p) p.addr)(P)) == map(λ(p) p.addr.city)(P) *)
+  (** The original version of T1 *)
+  Definition T1l P :=
     LAMap (LALambda "a" (LAUnop (ADot "city") (LAVar "a")))
-          (LAMap (LALambda "p" (LAUnop (ADot "addr") (LAVar "p"))) Q).
+          (LAMap (LALambda "p" (LAUnop (ADot "addr") (LAVar "p"))) P).
 
-  Definition T1r Q :=
-    LAMap (LALambda "p" (LAUnop (ADot "city") (LAUnop (ADot "addr") (LAVar "p")))) Q.
+  (** The simplified version of T1 *)
+  Definition T1r P :=
+    LAMap (LALambda "p" (LAUnop (ADot "city") (LAUnop (ADot "addr") (LAVar "p")))) P.
 
+
+  Lemma T1lr_equiv P : lalg_eq (T1l P) (T1r P).
+  Proof.
+    unfold lalg_eq, T1l, T1r.
+    intros.
+    autorewrite with lalg.
+    simpl.
+    unfold olift.
+    destruct (fun_of_lalg h0 env P); trivial.
+    unfold lift_oncoll.
+    destruct d; trivial.
+    induction l; simpl; trivial.
+    autorewrite with lalg.
+    case_eq (@fun_of_lalg TrivialModel.trivial_foreign_runtime h0
+             (@app
+                (prod string
+                   (@data (@foreign_runtime_data TrivialModel.trivial_foreign_runtime))) env
+                (@cons
+                   (prod string
+                      (@data (@foreign_runtime_data TrivialModel.trivial_foreign_runtime)))
+                   (@pair string
+                      (@data (@foreign_runtime_data TrivialModel.trivial_foreign_runtime))
+                      (String (Ascii.Ascii false false false false true true true false)
+                         EmptyString) a)
+                   (@nil
+                      (prod string
+                         (@data (@foreign_runtime_data TrivialModel.trivial_foreign_runtime))))))
+             (@LAUnop TrivialModel.trivial_foreign_runtime
+                (@ADot TrivialModel.trivial_foreign_data
+                   (@TrivialModel.trivial_foreign_unary_op TrivialModel.trivial_foreign_data)
+                   (String (Ascii.Ascii true false false false false true true false)
+                      (String (Ascii.Ascii false false true false false true true false)
+                         (String (Ascii.Ascii false false true false false true true false)
+                            (String
+                               (Ascii.Ascii false true false false true true true false)
+                               EmptyString)))))
+                (@LAVar TrivialModel.trivial_foreign_runtime
+                   (String (Ascii.Ascii false false false false true true true false)
+                           EmptyString)))); simpl; intros.
+    - unfold fun_of_lalg in H |- *.
+      rewrite H; clear H.
+      rewrite olift_some.
+      match_case_in IHl; intros; rewrite H in IHl.
+      + apply some_lift in H.
+        destruct H as [? ? ?]; subst.
+        apply lift_injective in IHl; [ | inversion 1; trivial].
+        rewrite <- IHl; clear IHl.
+        rewrite e.
+        simpl.
+        destruct ((@rmap (@data TrivialModel.trivial_foreign_data)
+                 (@data TrivialModel.trivial_foreign_data)
+                 (@fun_of_lalg_lambda TrivialModel.trivial_foreign_runtime h0 env
+                    (@LALambda TrivialModel.trivial_foreign_runtime
+                       (String (Ascii.Ascii true false false false false true true false)
+                          EmptyString)
+                       (@LAUnop TrivialModel.trivial_foreign_runtime
+                          (@ADot TrivialModel.trivial_foreign_data
+                             (@TrivialModel.trivial_foreign_unary_op
+                                TrivialModel.trivial_foreign_data)
+                             (String
+                                (Ascii.Ascii true true false false false true true false)
+                                (String
+                                   (Ascii.Ascii true false false true false true true false)
+                                   (String
+                                      (Ascii.Ascii false false true false true true true
+                                         false)
+                                      (String
+                                         (Ascii.Ascii true false false true true true true
+                                            false) EmptyString)))))
+                          (@LAVar TrivialModel.trivial_foreign_runtime
+                             (String
+                                (Ascii.Ascii true false false false false true true false)
+                                EmptyString))))) x)); simpl.
+        * autorewrite with lalg.
+          unfold fun_of_lalg.
+          simpl.
+          unfold edot.
+          rewrite @assoc_lookupr_app.
+          simpl.
+          trivial.
+        * repeat match_destr.
+      + symmetry in IHl.
+        apply none_lift in IHl.
+        apply none_lift in H.
+        rewrite H, IHl.
+        simpl.
+        destruct d; simpl; trivial.
+        match_destr.
+    - match_case; intros.
+      unfold fun_of_lalg in H, H0.
+      rewrite H in H0.
+      simpl in H0.
+      discriminate.
+  Qed.
+
+  
 (*  Eval vm_compute in (eval_q h T1l db1). *)
 (*  Eval vm_compute in (eval_q h T1r db1). *)
 (*  Eval vm_compute in (eval_nraenv_q h (algenv_of_lalg_lambda (q_to_lambda T1l)) db1). *)
 (*  Eval vm_compute in (eval_nraenv_q h (algenv_of_lalg_lambda (q_to_lambda T1r)) db1). *)
 
-  (* T2 : map(λ(x) x.age)(sel(λ(p) p.age > 25)(Q)) == sel(λ(a) a > 25)(map(λ(p) p.age)(Q)) *)
-  Definition T2l Q :=
+  (* T2 : map(λ(x) x.age)(sel(λ(p) p.age > 25)(P)) == sel(λ(a) a > 25)(map(λ(p) p.age)(P)) *)
+  Definition T2l P :=
     LAMap (LALambda "x" (LAUnop (ADot "age") (LAVar "x")))
           (LASelect (LALambda "p" (LABinop ALt
                                            (LAConst (dnat 25))
-                                           (LAUnop (ADot "age") (LAVar "p")))) Q).
+                                           (LAUnop (ADot "age") (LAVar "p")))) P).
 
-  Definition T2r Q :=
+  Definition T2r P :=
     LASelect (LALambda "a" (LABinop ALt
                                     (LAConst (dnat 25))
                                     (LAVar "a")))
-             (LAMap (LALambda "p" (LAUnop (ADot "age") (LAVar "p"))) Q).
+             (LAMap (LALambda "p" (LAUnop (ADot "age") (LAVar "p"))) P).
 
+  
 (*  Eval vm_compute in (eval_q h T2l db2). *)
   (* Eval vm_compute in (eval_q h T2r db2). *)
   (* Eval vm_compute in (eval_nraenv_q h (algenv_of_lalg_lambda (q_to_lambda T2l)) db2). *)
   (* Eval vm_compute in (eval_nraenv_q h (algenv_of_lalg_lambda (q_to_lambda T2r)) db2). *)
 
-  (* A1 : map(λ(p) [ person: p, kids: sel(λ(c) c.age > 25)(p.child) ])(Q) *)
+  (* A3 : map(λ(p) [ person: p, kids: sel(λ(c) c.age > 25)(p.child) ])(P) *)
 
-  Definition A1 Q :=
+  Definition A3 P :=
     LAMap
       (LALambda "p"
                 (LABinop AConcat (LAUnop (ARec "person") (LAVar "p"))
@@ -77,14 +176,14 @@ Section LambdaNRAExamples.
                                               (LABinop ALt
                                                        (LAConst (dnat 25))
                                                        (LAUnop (ADot "age") (LAVar "c"))))
-                                    (LAUnop (ADot "child") (LAVar "p")))))) Q.
+                                    (LAUnop (ADot "child") (LAVar "p")))))) P.
 
-  (* Eval vm_compute in (eval_q h A1 db2). *)
-  (* Eval vm_compute in (eval_nraenv_q h (algenv_of_lalg_lambda (q_to_lambda A1)) db2). *)
+  (* Eval vm_compute in (eval_q h A3 db2). *)
+  (* Eval vm_compute in (eval_nraenv_q h (algenv_of_lalg_lambda (q_to_lambda A3)) db2). *)
   
-  (* A2 : map(λ(p) [ person: p, kids: sel(λ(c) p.age > 25)(p.child) ])(Q) *)
+  (* A4 : map(λ(p) [ person: p, kids: sel(λ(c) p.age > 25)(p.child) ])(P) *)
 
-  Definition A2 Q :=
+  Definition A4 P :=
     LAMap
       (LALambda "p"
                 (LABinop AConcat (LAUnop (ARec "person") (LAVar "p"))
@@ -94,10 +193,10 @@ Section LambdaNRAExamples.
                                               (LABinop ALt
                                                        (LAConst (dnat 25))
                                                        (LAUnop (ADot "age") (LAVar "p"))))
-                                    (LAUnop (ADot "child") (LAVar "p")))))) Q.
+                                    (LAUnop (ADot "child") (LAVar "p")))))) P.
 
-  (* Eval vm_compute in (eval_q h A2 db2). *)
-  (* Eval vm_compute in (eval_nraenv_q h (algenv_of_lalg_lambda (q_to_lambda A2)) db2). *)
+  (* Eval vm_compute in (eval_q h A4 db2). *)
+  (* Eval vm_compute in (eval_nraenv_q h (algenv_of_lalg_lambda (q_to_lambda A4)) db2). *)
 
 End LambdaNRAExamples.
 
