coq/Frontend/LambdaNRA/LambdaAlgEq.v
@@ -1,0 +1,164 @@
+Require Import String.
+Require Import List.
+Require Import Arith.
+Require Import EquivDec.
+Require Import Morphisms.
+
+Require Import Utils BasicRuntime.
+
+Require Import LambdaAlg.
+Section LambdaNRAEq.
+
+  Context {fruntime:foreign_runtime}.
+
+    Definition lalg_eq (op1 op2:lalg) : Prop :=
+    forall
+      (h:list(string*string))
+      (env:bindings)
+      (dn_env:Forall (fun d => data_normalized h (snd d)) env),
+       fun_of_lalg h env op1 = fun_of_lalg h env op2.
+
+    Definition lalg_lambda_eq (op1 op2:lalg_lambda) : Prop :=
+    forall
+      (h:list(string*string))
+      (env:bindings)
+      (dn_env:Forall (fun d => data_normalized h (snd d)) env)
+      (d:data)
+      (dn_d:data_normalized h d),
+      fun_of_lalg_lambda h env op1 d = fun_of_lalg_lambda h env op2 d.
+
+  Global Instance lalg_equiv : Equivalence lalg_eq.
+  Proof.
+    constructor.
+    - unfold Reflexive, lalg_eq.
+      intros; reflexivity.
+    - unfold Symmetric, lalg_eq.
+      intros. rewrite (H h env dn_env) by trivial; reflexivity.
+    - unfold Transitive, lalg_eq.
+      intros. rewrite (H h env dn_env) by trivial; rewrite (H0 h env dn_env) by trivial; reflexivity.
+  Qed.
+
+  Global Instance lalg_lambda_equiv : Equivalence lalg_lambda_eq.
+  Proof.
+    constructor.
+    - unfold Reflexive, lalg_lambda_eq.
+      intros; reflexivity.
+    - unfold Symmetric, lalg_lambda_eq.
+      intros. rewrite (H h env dn_env) by trivial; reflexivity.
+    - unfold Transitive, lalg_lambda_eq.
+      intros. rewrite (H h env dn_env) by trivial; rewrite (H0 h env dn_env) by trivial; reflexivity.
+  Qed.
+
+  Global Instance lavar_proper : Proper (eq ==> lalg_eq) LAVar.
+  Proof.
+    unfold Proper, respectful, lalg_eq; intros.
+    subst.
+    reflexivity.
+  Qed.
+
+  Global Instance laconst_proper : Proper (eq ==> lalg_eq) LAConst.
+  Proof.
+    unfold Proper, respectful, lalg_eq; intros.
+    subst.
+    reflexivity.
+  Qed.
+
+  Global Instance labinop_proper :
+    Proper (eq ==> lalg_eq ==> lalg_eq ==> lalg_eq) LABinop.
+  Proof.
+    unfold Proper, respectful, lalg_eq; intros.
+    subst.
+    cbn.
+    rewrite <- H0, H1 by trivial.
+    reflexivity.
+  Qed.
+
+  Global Instance launop_proper :
+    Proper (eq ==> lalg_eq ==> lalg_eq) LAUnop.
+  Proof.
+    unfold Proper, respectful, lalg_eq; intros.
+    subst.
+    cbn.
+    rewrite <- H0 by trivial.
+    reflexivity.
+  Qed.
+
+  Global Instance lamap_proper :
+    Proper (lalg_lambda_eq ==> lalg_eq ==> lalg_eq) LAMap.
+  Proof.
+    unfold Proper, respectful, lalg_eq, lalg_lambda_eq; intros.
+    autorewrite with lalg.
+    rewrite <- H0 by trivial.
+    apply olift_ext; intros.
+    apply lift_oncoll_ext; intros; subst.
+    f_equal.
+    apply rmap_ext; intros.
+    apply H; trivial.
+    eapply fun_of_lalg_normalized in H1; trivial.
+    invcs H1.
+    rewrite Forall_forall in H4.
+    eauto.
+  Qed.
+
+  Global Instance lamapconcat_proper :
+    Proper (lalg_lambda_eq ==> lalg_eq ==> lalg_eq) LAMapConcat.
+  Proof.
+    unfold Proper, respectful, lalg_eq, lalg_lambda_eq; intros.
+    autorewrite with lalg.
+    rewrite <- H0 by trivial.
+    apply olift_ext; intros.
+    apply lift_oncoll_ext; intros; subst.
+    f_equal.
+    apply rmap_concat_ext; intros.
+    apply H; trivial.
+    eapply fun_of_lalg_normalized in H1; trivial.
+    invcs H1.
+    rewrite Forall_forall in H4.
+    eauto.
+  Qed.
+  
+  Global Instance laproduct_proper :
+    Proper (lalg_eq ==> lalg_eq ==> lalg_eq) LAProduct.
+  Proof.
+    unfold Proper, respectful, lalg_eq, lalg_lambda_eq; intros.
+    autorewrite with lalg.
+    simpl.
+    rewrite <- H, H0 by trivial.
+    trivial.
+  Qed.
+
+  Global Instance laselect_proper :
+    Proper (lalg_lambda_eq ==> lalg_eq ==> lalg_eq) LASelect.
+  Proof.
+    unfold Proper, respectful, lalg_eq, lalg_lambda_eq; intros.
+    autorewrite with lalg.
+    rewrite <- H0 by trivial.
+    apply olift_ext; intros.
+    apply lift_oncoll_ext; intros; subst.
+    f_equal.
+    apply lift_filter_ext; intros.
+    rewrite H; trivial.
+    eapply fun_of_lalg_normalized in H1; trivial.
+    invcs H1.
+    rewrite Forall_forall in H4.
+    eauto.
+  Qed.
+
+  Global Instance lalambda_proper :
+    Proper (eq ==> lalg_eq ==> lalg_lambda_eq) LALambda.
+  Proof.
+    unfold Proper, respectful, lalg_eq, lalg_lambda_eq; intros.
+    subst.
+    autorewrite with lalg.
+    rewrite H0.
+    - reflexivity.
+    - apply Forall_app; auto.
+  Qed.
+
+End LambdaNRAEq.
+
+(* 
+*** Local Variables: ***
+*** coq-load-path: (("../../../coq" "QCert")) ***
+*** End: ***
+*)
